Semantics/ReflTransRel.lean
@@ -1,7 +1,7 @@
 -- Reflexive transitive relations
-inductive ReflTrans (r: α -> α -> Prop): α -> α -> Prop
+inductive ReflTrans (r: α → α → Prop): α → α → Prop
   | refl: ReflTrans r a a
-  | tail: ReflTrans r a b -> r b c -> ReflTrans r a c
+  | tail: ReflTrans r a b → r b c → ReflTrans r a c
 
 namespace ReflTrans
 
@@ -18,16 +18,16 @@ theorem head (hab: r a b) (hbc: ReflTrans r b c): ReflTrans r a c := by
   | refl => exact tail refl hab
   | tail _ hcd hac => exact tail hac hcd
 
-theorem head_induction_on {P: ∀a: α, ReflTrans r a b -> Prop} {a: α} (h: ReflTrans r a b)
+theorem head_induction_on {P: ∀a: α, ReflTrans r a b → Prop} {a: α} (h: ReflTrans r a b)
     (refl: P b refl)
-    (head: ∀{a c} (h': r a c) (h: ReflTrans r c b), P c h -> P a (head h' h)): P a h := by
+    (head: ∀{a c} (h': r a c) (h: ReflTrans r c b), P c h → P a (head h' h)): P a h := by
   induction h with
   | refl => exact refl
   | tail _ hbc ih =>
     exact ih (head hbc _ refl) (fun h1 h2 => head h1 (tail h2 hbc))
 
-theorem lift {r: α -> α -> Prop} {p: β -> β -> Prop} {a b: α} (f: α -> β)
-    (h: ∀{a b}, r a b -> p (f a) (f b)) (hab: ReflTrans r a b): ReflTrans p (f a) (f b) := by
+theorem lift {r: α → α → Prop} {p: β → β → Prop} {a b: α} (f: α → β)
+    (h: ∀{a b}, r a b → p (f a) (f b)) (hab: ReflTrans r a b): ReflTrans p (f a) (f b) := by
   induction hab with
   | refl => exact refl
   | tail _hab hbc ih => exact tail ih (h hbc)
