Semantics/Imp/SmallStep.lean
@@ -3,8 +3,8 @@ import Semantics.ReflTransRel
 
 namespace Com
 
-inductive SmallStep: Com × State -> Com × State -> Prop where
-  | ass: SmallStep (ass v a, s) ({}, s[v <- a s])
+inductive SmallStep: Com × State → Com × State → Prop where
+  | ass: SmallStep (ass v a, s) ({}, s[v ← a s])
   | skipCat: SmallStep ({}++c, s) (c, s)
   | cat (hstep: SmallStep (c, s) (c', s')):
     SmallStep (c++c'', s) (c'++c'', s')
@@ -17,10 +17,10 @@ infixl:10 " ~> " => SmallStep
 namespace SmallStep
 
 private example: ([|x = 1; while x <= 2 {x = x + 1}|], s0) ~>
-  ([|skip; while x <= 2 {x = x + 1}|], s0["x" <- 1]) := cat ass
+  ([|skip; while x <= 2 {x = x + 1}|], s0["x" ← 1]) := cat ass
 
 theorem cat_eq: ((c++c'', s) ~> conf)
-  <-> ((∃c' s', ((c, s) ~> (c', s')) ∧ conf = (c'++c'', s'))
+  ↔ ((∃c' s', ((c, s) ~> (c', s')) ∧ conf = (c'++c'', s'))
     ∨ (c = {} ∧ conf = (c'', s))) := {
     mp := fun hmp => match hmp with
       | skipCat => Or.inr ⟨rfl, rfl⟩
@@ -31,7 +31,7 @@ theorem cat_eq: ((c++c'', s) ~> conf)
   }
 
 theorem cond_eq: ((.ifElse b c c', s) ~> conf)
-  <-> (b s ∧ conf = (c, s) ∨ b s = false ∧ conf = (c', s)) := {
+  ↔ (b s ∧ conf = (c, s) ∨ b s = false ∧ conf = (c', s)) := {
     mp := fun hmp => match hb: b s with
       | false => match hmp with | ifElse => Or.inr ⟨rfl, hb ▸ rfl⟩
       | true => match hmp with | ifElse => Or.inl ⟨rfl, hb ▸ rfl⟩,
@@ -43,25 +43,25 @@ theorem cond_eq: ((.ifElse b c c', s) ~> conf)
   }
 
 theorem cond_false (hb: b s = false): ((.ifElse b c c', s) ~> conf)
-  <-> (conf = (c', s)) := by
+  ↔ (conf = (c', s)) := by
   rw [cond_eq, hb]
   exact ⟨fun (Or.inr ⟨rfl, h⟩) => h, (Or.inr ⟨rfl, .⟩)⟩
 
 infixl:10 " ~>* " => ReflTrans SmallStep
 
 private example: ([|x = 1; while x <= 1 {x = x + 1}|], s0) ~>*
-    ({}, s0["x" <- 1]["x" <- 2]) := by
+    ({}, s0["x" ← 1]["x" ← 2]) := by
   apply ReflTrans.head (cat ass) (ReflTrans.head skipCat _)
   apply ReflTrans.head whileLoop
-  have hs : s0["x" <- Aexp.eval 1 s0] = s0["x" <- 1] := rfl
-  have hcond : (Bexp.le (Aexp.var "x") 1) (s0["x" <- 1]) = true := rfl
+  have hs : s0["x" ← Aexp.eval 1 s0] = s0["x" ← 1] := rfl
+  have hcond : (Bexp.le (Aexp.var "x") 1) (s0["x" ← 1]) = true := rfl
   rw [hs, hcond]
   apply ReflTrans.head (cat ass)
   apply ReflTrans.head skipCat
   apply ReflTrans.head whileLoop
-  have hs : s0["x" <- 1]["x" <- (Aexp.var "x" + 1) (s0["x" <- 1])] =
-    s0["x" <- 1]["x" <- 2] := rfl
-  have hcond : (Bexp.le (Aexp.var "x") 1) (s0["x" <- 1]["x" <- 2])
+  have hs : s0["x" ← 1]["x" ← (Aexp.var "x" + 1) (s0["x" ← 1])] =
+    s0["x" ← 1]["x" ← 2] := rfl
+  have hcond : (Bexp.le (Aexp.var "x") 1) (s0["x" ← 1]["x" ← 2])
     = false := rfl
   rw [hs, hcond]
   apply ReflTrans.refl
